Soundness (WIP)

src/MicroSail/Symbolic/Sound.v
@@ -137,16 +137,15 @@ Module Soundness
       represents ι (symbolicstate_assume_formula fml s__sym) s__sc.
     Proof. unfold represents; destruct s__sym, s__sc; cbn; intuition. Qed.
 
-    Lemma represents_produce_chunk {Γ Σ} (ι : SymInstance Σ) (c : Chunk Σ)
+    Lemma represents_produce_chunk {Γ Σ} (ι : SymInstance Σ) (c1 : Chunk Σ) (c2 : SCChunk)
           (s__sym : SymbolicState Γ Σ) (s__sc : SCState Γ) :
-      represents ι s__sym s__sc <->
-      represents ι (symbolicstate_produce_chunk c s__sym) (scstate_produce_chunk (inst ι c) s__sc).
+      represents ι s__sym s__sc /\ c2 = inst ι c1 <->
+      represents ι (symbolicstate_produce_chunk c1 s__sym) (scstate_produce_chunk c2 s__sc).
     Proof.
       unfold represents; destruct s__sym, s__sc; cbn - [inst].
-      change (inst ι (cons c ?h)) with (cons (inst ι c) (inst ι h)).
-      apply and_iff_compat_r.
-      split; intros; subst; auto.
-      now dependent elimination H.
+      change (inst ι (cons c1 ?h)) with (cons (inst ι c1) (inst ι h)).
+      split; intros H; destruct_propositional H; subst; intuition.
+      now dependent elimination H1.
     Qed.
 
     Lemma inst_subst_formula {Σ1 Σ2} (ι : SymInstance Σ2) (ζ : Sub Σ1 Σ2) (fml : Formula Σ1) :
@@ -290,10 +289,11 @@ Module Soundness
     Definition stateprop_lift {Γ AT A Σ} {instA : Inst AT A} (ι : SymInstance Σ) (POST : A -> SCState Γ -> Prop) :
       StateProperty Γ AT Σ :=
       fun Σ1 ζ1 v1 s__sym1 =>
-        forall ι1 s__sc1,
+        forall ι1,
           syminstance_rel ζ1 ι ι1 ->
-          represents ι1 s__sym1 s__sc1 ->
-          POST (inst ι1 v1) s__sc1.
+          forall s__sc1,
+            represents ι1 s__sym1 s__sc1 ->
+            POST (inst ι1 v1) s__sc1.
 
     Lemma stateprop_lift_dcl {Γ AT A Σ} `{InstLaws AT A} (ι : SymInstance Σ) (POST : A -> SCState Γ -> Prop) :
       stateprop_downwards_closed (stateprop_lift ι POST).
@@ -301,40 +301,104 @@ Module Soundness
       unfold stateprop_downwards_closed, stateprop_lift; intros.
       rewrite inst_subst.
       apply syminstance_rel_comp in H4.
-      apply (H3 (inst ι1 ζ2) s__sc1).
+      apply (H3 (inst ι1 ζ2)).
       - assumption.
       - revert H5. now apply represents_rel.
     Qed.
 
-    Definition approximates {Γ1 Γ2 AT A Σ} `{instA : Inst AT A} (ι : SymInstance Σ)
-               (dm : DynamicMutator Γ1 Γ2 AT Σ) (sm : SCMut Γ1 Γ2 A) : Prop :=
-      forall (s__sym : SymbolicState Γ1 Σ) (s__sc : SCState Γ1) (POST : A -> SCState Γ2 -> Prop),
-        represents ι s__sym s__sc ->
-        dmut_wp dm (stateprop_lift ι POST) s__sym ->
-        scmut_wp sm POST s__sc.
+    Definition APPROX Γ1 Γ2 AT A {instA : Inst AT A} : Type :=
+      forall Σ (ι : SymInstance Σ),
+        DynamicMutator Γ1 Γ2 AT Σ -> SCMut Γ1 Γ2 A -> Prop.
+    Arguments APPROX _ _ _ _ {_}.
+
+    Definition box {Γ1 Γ2 AT A} {instA : Inst AT A} (R : APPROX Γ1 Γ2 AT A) : APPROX Γ1 Γ2 AT A :=
+      fun Σ ι dm sm =>
+        forall Σ1 (ζ1 : Sub Σ Σ1) (ι1 : SymInstance Σ1),
+          syminstance_rel ζ1 ι ι1 ->
+          R Σ1 ι1 (dmut_sub ζ1 dm) sm.
+
+    Lemma box_proj {Γ1 Γ2 AT A} {instA : Inst AT A} (R : APPROX Γ1 Γ2 AT A) :
+      forall Σ (ι : SymInstance Σ) dm sm,
+        box R ι dm sm -> R _ ι dm sm.
+    Proof.
+      intros ? ? ? ? b.
+      unfold box in b.
+      inster b by apply syminstance_rel_refl.
+      unfold dmut_sub in b.
+      (* apply b. *)
+    Admitted.
+
+    Definition box_box {Γ1 Γ2 AT A} {instA : Inst AT A} (R : APPROX Γ1 Γ2 AT A) :
+      forall Σ (ι : SymInstance Σ) dm sm,
+        box R ι dm sm -> box (box R) ι dm sm.
+    Proof.
+      intros ? ? ? ?. unfold box. intros bb Σ1 ζ1 ι1 ? Σ2 ζ2 ι2 ?.
+      specialize (bb Σ2 (sub_comp ζ1 ζ2) ι2).
+      inster bb by eapply syminstance_rel_trans; eauto.
+      (* apply bb. *)
+    Admitted.
+
+    Definition approximates {Γ1 Γ2 AT A} {instA : Inst AT A} : APPROX Γ1 Γ2 AT A :=
+      fun Σ ι dm sm =>
+        forall (s__sym : SymbolicState Γ1 Σ) (s__sc : SCState Γ1),
+          represents ι s__sym s__sc ->
+          forall (POST : A -> SCState Γ2 -> Prop),
+            dmut_wp dm (stateprop_lift ι POST) s__sym ->
+            scmut_wp sm POST s__sc.
+
+    Lemma approximates_proj {Γ1 Γ2 AT A} {instA : Inst AT A} {Σ} (ι : SymInstance Σ)
+      (dm : DynamicMutator Γ1 Γ2 AT Σ) (sm : SCMut Γ1 Γ2 A) :
+      box approximates ι dm sm -> approximates ι dm sm.
+    Proof.
+      unfold approximates, box. intros.
+      inster H by apply syminstance_rel_refl.
+      inster H by eauto. apply H. clear H.
+      unfold dmut_wp, dmut_sub in *. intros Σ1 ζ1.
+      rewrite sub_comp_id_left. apply H1.
+    Qed.
+
+    Lemma approximates_box_box {Γ1 Γ2 AT A} {instA : Inst AT A} {Σ} (ι : SymInstance Σ)
+      (dm : DynamicMutator Γ1 Γ2 AT Σ) (sm : SCMut Γ1 Γ2 A) :
+      box approximates ι dm sm -> box (box approximates) ι dm sm.
+    Proof.
+      unfold approximates, box, dmut_wp, dmut_sub. intros.
+      inster H by eapply syminstance_rel_trans; eauto.
+      inster H by eauto. apply H. clear H. intros. now rewrite sub_comp_assoc.
+    Qed.
+
+    Lemma approximates_sub {Γ Σ Σ1} (ζ1 : Sub Σ Σ1) (ι : SymInstance Σ) (ι1 : SymInstance Σ1)
+      (relι1 : syminstance_rel ζ1 ι ι1) (d : DynamicMutator Γ Γ Unit Σ) (s : SCMut Γ Γ unit) :
+      box approximates ι d s -> box approximates ι1 (dmut_sub ζ1 d) s.
+    Proof. intros H. eapply approximates_box_box; eauto. Qed.
 
     Lemma scmut_wp_demonic_binary {Γ1 Γ2 A} (sm1 sm2 : SCMut Γ1 Γ2 A) (s__sc : SCState Γ1) (POST : A -> SCState Γ2 -> Prop) :
-      scmut_wp (scmut_demonic_binary sm1 sm2) POST s__sc <-> scmut_wp sm1 POST s__sc /\ scmut_wp sm2 POST s__sc.
+      scmut_wp (scmut_demonic_binary sm1 sm2) POST s__sc <->
+      scmut_wp sm1 POST s__sc /\ scmut_wp sm2 POST s__sc.
     Proof. unfold scmut_wp, scmut_demonic_binary; cbn; intuition. Qed.
 
     Lemma dmut_wp_demonic_binary {Γ1 Γ2 Σ A} (m1 m2 : DynamicMutator Γ1 Γ2 A Σ)
-      (POST : forall Σ', Sub Σ Σ' -> A Σ' -> SymbolicState Γ2 Σ' -> Prop) (s : SymbolicState Γ1 Σ) :
+      (POST : StateProperty Γ2 A Σ) (s : SymbolicState Γ1 Σ) :
         dmut_wp (dmut_demonic_binary m1 m2) POST s <->
         dmut_wp m1 POST s /\ dmut_wp m2 POST s.
     Proof. unfold dmut_wp, dmut_demonic_binary; cbn; intuition. Qed.
 
+    Lemma dmut_wp_sub_demonic_binary {Γ1 Γ2 Σ A Σ1} (ζ1 : Sub Σ Σ1) (m1 m2 : DynamicMutator Γ1 Γ2 A Σ)
+      (POST : StateProperty Γ2 A Σ1) (s : SymbolicState Γ1 Σ1) :
+        dmut_wp (dmut_sub ζ1 (dmut_demonic_binary m1 m2)) POST s <->
+        dmut_wp (dmut_sub ζ1 m1) POST s /\ dmut_wp (dmut_sub ζ1 m2) POST s.
+    Proof. unfold dmut_wp, dmut_demonic_binary; cbn; intuition. Qed.
+
     Lemma approximates_demonic_binary {Γ1 Γ2 Σ} (ι : SymInstance Σ)
           (dm1 dm2 : DynamicMutator Γ1 Γ2 Unit Σ) (sm1 sm2 : SCMut Γ1 Γ2 unit) :
-      approximates ι dm1 sm1 ->
-      approximates ι dm2 sm2 ->
-      approximates ι (dmut_demonic_binary dm1 dm2) (scmut_demonic_binary sm1 sm2).
+      box approximates ι dm1 sm1 ->
+      box approximates ι dm2 sm2 ->
+      box approximates ι (dmut_demonic_binary dm1 dm2) (scmut_demonic_binary sm1 sm2).
     Proof.
-      intros H1 H2 ? ? ? H__s H.
-      apply scmut_wp_demonic_binary.
-      apply dmut_wp_demonic_binary in H.
-      split.
-      now apply (H1 _ _ _ H__s).
-      now apply (H2 _ _ _ H__s).
+      unfold box. intros H1 H2 Σ1 ζ1 ι1 H__ι.
+      specialize (H1 Σ1 ζ1 ι1 H__ι). specialize (H2 Σ1 ζ1 ι1 H__ι).
+      intros ? ? H__s POST. specialize (H1 _ _ H__s POST). specialize (H2 _ _ H__s POST).
+      intros H. apply dmut_wp_sub_demonic_binary in H. destruct H.
+      apply scmut_wp_demonic_binary. split; auto.
     Qed.
 
     Lemma scmut_wp_demonic {Γ1 Γ2 A B} (sm : B -> SCMut Γ1 Γ2 A) (s__sc : SCState Γ1) (POST : A -> SCState Γ2 -> Prop) :
@@ -347,62 +411,80 @@ Module Soundness
         forall b, dmut_wp (m b) POST s.
     Proof. unfold dmut_wp, dmut_demonic; cbn; intuition. Qed.
 
-    Lemma dmut_wp_produce_chunk {Γ Σ} (c : Chunk Σ) (s__sym : SymbolicState Γ Σ)
-          (POST : StateProperty Γ Unit Σ) (POST_dcl : stateprop_downwards_closed POST) :
-      dmut_wp (dmut_produce_chunk c) POST s__sym <->
-      POST Σ (sub_id Σ) tt (symbolicstate_produce_chunk c s__sym).
+    Lemma apply_sprop_dcl {Γ Σ A} `{Subst A} (p : StateProperty Γ A Σ) (pdcl : stateprop_downwards_closed p) :
+      forall Σ1 Σ2 (ζ1 : Sub Σ Σ1) (ζ2 : Sub Σ1 Σ2) (ζ12 : Sub Σ Σ2)
+        (a1 : A Σ1) (s1 : SymbolicState Γ Σ1),
+        ζ12 = sub_comp ζ1 ζ2 ->
+        p Σ1 ζ1 a1 s1 ->
+        p Σ2 ζ12 (subst ζ2 a1) (subst ζ2 s1).
+    Proof. intros. subst. now apply pdcl. Qed.
+
+    Lemma subst_symbolicstate_produce_chunk {Γ Σ Σ1} (ζ1 : Sub Σ Σ1) (c : Chunk Σ) (s : SymbolicState Γ Σ) :
+      subst ζ1 (symbolicstate_produce_chunk c s) = symbolicstate_produce_chunk (subst ζ1 c) (subst ζ1 s).
+    Proof. now destruct s. Qed.
+
+    Lemma dmut_wp_produce_chunk {Γ Σ Σ1} (ζ1 : Sub Σ Σ1) (c : Chunk _) (s__sym : SymbolicState Γ _)
+          (POST : StateProperty Γ Unit _) (POST_dcl : stateprop_downwards_closed POST) :
+      dmut_wp (dmut_sub ζ1 (dmut_produce_chunk c)) POST s__sym <->
+      POST Σ1 (sub_id Σ1) tt (symbolicstate_produce_chunk (subst ζ1 c) s__sym).
     Proof.
       split.
-      - intros dwp. specialize (dwp Σ (sub_id Σ)). cbn in dwp.
-        now rewrite ?sub_comp_id_left, ?subst_sub_id in dwp.
-      - intros ? ? ?. cbn.
-        replace (symbolicstate_produce_chunk (subst ζ1 c) (subst ζ1 s__sym))
-          with (subst ζ1 (symbolicstate_produce_chunk c s__sym)) by now destruct s__sym.
-        replace (sub_comp ζ1 (sub_id Σ1)) with (sub_comp (sub_id Σ) ζ1)
-          by now rewrite sub_comp_id_right, sub_comp_id_left.
-        now apply POST_dcl.
+      - intros dwp.
+        specialize (dwp Σ1 (sub_id Σ1)). cbn in dwp.
+        now rewrite ?sub_comp_id_right, ?subst_sub_id in dwp.
+      - intros p Σ2 ζ2. cbn. rewrite subst_sub_comp. revert p.
+        rewrite <- subst_symbolicstate_produce_chunk.
+        rewrite sub_comp_id_right. change tt with (subst ζ2 tt).
+        apply apply_sprop_dcl; auto. now rewrite sub_comp_id_left.
     Qed.
 
     Lemma dmut_produce_chunk_sound {Γ Σ} (ι : SymInstance Σ) (c : Chunk Σ) :
-      approximates
+      box approximates
         (Γ1 := Γ) (Γ2 := Γ) ι
         (dmut_produce_chunk c)
         (scmut_produce_chunk (inst ι c)).
     Proof.
-      intros ? ? ? Hrep dwp. cbn.
+      intros ? ? ? ? ? ? Hrep ? dwp. cbn.
       apply dmut_wp_produce_chunk in dwp; auto using stateprop_lift_dcl.
-      apply (dwp ι); auto using syminstance_rel_refl.
-      now apply represents_produce_chunk.
+      apply (dwp ι1); auto using syminstance_rel_refl.
+      apply represents_produce_chunk; split; auto.
+      rewrite inst_subst. unfold syminstance_rel in H. now subst.
     Qed.
 
     Lemma dmut_assume_formula_sound {Γ Σ} (ι : SymInstance Σ) (fml : Formula Σ) :
-      approximates
+      box approximates
         (Γ1 := Γ) (Γ2 := Γ) ι
         (dmut_assume_formula fml)
         (scmut_assume_formula ι fml).
     Proof.
-      intros ? ? ? H__state H.
-      unfold dmut_wp, dmut_assume_formula in H.
-      specialize (H Σ (sub_id Σ)).
-      rewrite subst_sub_id in H.
-      destruct (try_solve_formula_spec (ι := ι) fml) as [? H1|_].
-      - intros ->%H1. clear H1. cbn in *.
-        rewrite subst_sub_id, sub_comp_id_left in H.
-        refine (H _ _ _ H__state).
-        apply syminstance_rel_refl.
-      - destruct fml; cbn in *; intros;
+      intros ? ? ? ? ? ? H__state POST H.
+      unfold dmut_wp, dmut_sub, dmut_assume_formula in H.
+      specialize (H Σ1 (sub_id Σ1)).
+      rewrite sub_comp_id_right in H.
+      unfold scmut_wp, scmut_assume_formula. cbn. intros.
+      destruct (try_solve_formula_spec (ι := ι1) (subst ζ1 fml)).
+      - assert (a=true) by admit. subst a. cbn in H.
+        rewrite ?subst_sub_id, ?sub_comp_id_left in H.
+        unfold stateprop_lift in H.
+        inster H by apply syminstance_rel_refl.
+        now apply H.
+      - cbn in H. unfold stateprop_lift in H.
+        destruct fml; cbn in *; intros;
           rewrite ?subst_sub_id, ?sub_comp_id_left in H.
-        + apply (H _ _ (syminstance_rel_refl ι)).
-          now apply represents_assume_formula.
-        + apply (H _ _ (syminstance_rel_refl ι)).
-          now apply represents_assume_formula.
-        + destruct s__sc as [δ__sc h__sc].
+        + inster H by apply syminstance_rel_refl. apply H.
+          apply represents_assume_formula. split; cbn; auto.
           admit.
-        + apply (H _ _ (syminstance_rel_refl ι)).
-          now apply represents_assume_formula.
+        + inster H by apply syminstance_rel_refl. apply H.
+          apply represents_assume_formula. split; cbn; auto.
+          rewrite inst_subst. unfold syminstance_rel in H0.
+          now subst.
+        + admit.
+        + inster H by apply syminstance_rel_refl. apply H.
+          apply represents_assume_formula. split; cbn; auto.
+          admit.
     Admitted.
 
-    Opaque dmut_assume_formula.
+    (* Opaque dmut_assume_formula. *)
 
     Definition dmut_wf {Γ1 Γ2 A Σ0} `{Subst A} (d : DynamicMutator Γ1 Γ2 A Σ0) : Prop :=
       forall Σ1 Σ2 (ζ1 : Sub Σ0 Σ1) (ζ2 : Sub Σ1 Σ2) (s1 : SymbolicState Γ1 Σ1)
@@ -548,76 +630,81 @@ Module Soundness
       (dmf : forall Σ1, Sub Σ0 Σ1 -> AT Σ1 -> DynamicMutator Γ2 Γ3 BT Σ1)
       (dmf_wf : forall Σ1 ζ a, dmut_wf (dmf Σ1 ζ a))
       (smf : A -> SCMut Γ2 Γ3 B) :
-      approximates ι0 dma sma ->
+      box approximates ι0 dma sma ->
       (forall Σ1 (ζ1 : Sub Σ0 Σ1) (a1 : AT Σ1) (ι1 : SymInstance Σ1),
           syminstance_rel ζ1 ι0 ι1 ->
-          approximates ι1 (dmf Σ1 ζ1 a1) (smf (inst ι1 a1))) ->
-      approximates ι0 (dmut_bind dma dmf) (scmut_bind sma smf).
-    Proof.
-      intros H__a H__f s__sym0 s__sc0 POST H__rep H__wp.
-      apply scmut_wp_bind.
-      apply dmut_wp_bind in H__wp; auto using stateprop_lift_dcl.
-      apply H__a with s__sym0. assumption.
-      revert H__wp. apply dmut_wp_monotonic.
-      intros Σ1 ζ1 a1 s__sym1 H__wp ι1 s__sc1 ι__rel1 s__rep1.
-      apply (H__f Σ1 ζ1 a1 ι1 ι__rel1 s__sym1). assumption.
-      revert H__wp. apply dmut_wp_monotonic.
-      intros Σ2 ζ2 b2 s__sym2 H__post ι2 s__sc2 ι__rel2 s__rep2.
-      apply H__post. apply (syminstance_rel_trans ι__rel1 ι__rel2). assumption.
-    Qed.
+          box approximates ι1 (dmf Σ1 ζ1 a1) (smf (inst ι1 a1))) ->
+      box approximates ι0 (dmut_bind dma dmf) (scmut_bind sma smf).
+    (* Proof. *)
+    (*   intros H__a H__f. *)
+    (*   intros Σ1 ζ1 ι1 relι1 s__sym1 s__sc1 H__rep POST H__wp. *)
+    (*   apply scmut_wp_bind. *)
+    (*   apply dmut_wp_bind in H__wp; auto using stateprop_lift_dcl. *)
+    (*   apply H__a with s__sym0. assumption. *)
+    (*   revert H__wp. apply dmut_wp_monotonic. *)
+    (*   intros Σ1 ζ1 a1 s__sym1 H__wp ι1 s__sc1 ι__rel1 s__rep1. *)
+    (*   apply (H__f Σ1 ζ1 a1 ι1 ι__rel1 s__sym1). assumption. *)
+    (*   revert H__wp. apply dmut_wp_monotonic. *)
+    (*   intros Σ2 ζ2 b2 s__sym2 H__post ι2 s__sc2 ι__rel2 s__rep2. *)
+    (*   apply H__post. apply (syminstance_rel_trans ι__rel1 ι__rel2). assumption. *)
+    (* Qed. *)
+    Admitted.
 
     Lemma dmut_fresh_sound {Γ Σ ς τ} (ι : SymInstance Σ)
           (dm : DynamicMutator Γ Γ Unit (Σ ▻ (ς,τ))) (wfdm : dmut_wf dm)
           (sm : Lit τ -> SCMut Γ Γ unit) :
-      (forall v, approximates (env_snoc ι _ v) dm (sm v)) ->
-      approximates ι
+      (forall v, box approximates (env_snoc ι _ v) dm (sm v)) ->
+      box approximates ι
         (dmut_fresh (ς,τ) dm)
         (scmut_demonic sm).
-    Proof.
-      intros HYP.
-      unfold approximates; cbn.
-      intros ? ? ? H__state H.
-      apply scmut_wp_demonic. intros v.
-      apply (HYP v (subst sub_wk1 s__sym) s__sc POST).
-      - revert H__state. clear.
-        apply represents_rel.
-        apply syminstance_rel_wk1.
-      - apply (@dmut_wp_fresh Γ Σ Unit ς τ SubstUnit) in H.
-        + revert H; clear.
-          apply dmut_wp_monotonic; cbn; intros ? ? []; intros.
-          dependent elimination ζ as [@env_snoc Σ0 ζ _ t].
-          unfold stateprop_specialize in H.
-          rewrite sub_comp_wk1_tail in H; cbn in *.
-          intros ι1 s1 H0 H1.
-          apply H.
-          * now apply syminstance_rel_snoc in H0.
-          * assumption.
-        + apply stateprop_lift_dcl.
-        + assumption.
-    Qed.
+    (* Proof. *)
+    (*   intros HYP. *)
+    (*   unfold approximates; cbn. *)
+    (*   intros ? ? ? H__state H. *)
+    (*   apply scmut_wp_demonic. intros v. *)
+    (*   apply (HYP v (subst sub_wk1 s__sym) s__sc POST). *)
+    (*   - revert H__state. clear. *)
+    (*     apply represents_rel. *)
+    (*     apply syminstance_rel_wk1. *)
+    (*   - apply (@dmut_wp_fresh Γ Σ Unit ς τ SubstUnit) in H. *)
+    (*     + revert H; clear. *)
+    (*       apply dmut_wp_monotonic; cbn; intros ? ? []; intros. *)
+    (*       dependent elimination ζ as [@env_snoc Σ0 ζ _ t]. *)
+    (*       unfold stateprop_specialize in H. *)
+    (*       rewrite sub_comp_wk1_tail in H; cbn in *. *)
+    (*       intros ι1 s1 H0 H1. *)
+    (*       apply H. *)
+    (*       * now apply syminstance_rel_snoc in H0. *)
+    (*       * assumption. *)
+    (*     + apply stateprop_lift_dcl. *)
+    (*     + assumption. *)
+    (* Qed. *)
+    Admitted.
 
     Lemma dmut_produce_sound {Γ Σ} (asn : Assertion Σ) (ι : SymInstance Σ) :
-      approximates
+      box approximates
         (Γ1 := Γ) (Γ2 := Γ) ι
         (dmut_produce asn)
         (scmut_produce ι asn).
     Proof.
       induction asn; cbn.
-      - apply dmut_assume_formula_sound.
+      - admit.
+        (* apply dmut_assume_formula_sound. *)
       - apply dmut_produce_chunk_sound.
       - apply approximates_demonic_binary.
         + unfold dmut_bind_right.
           eapply dmut_bind_sound. admit. admit.
           apply dmut_assume_formula_sound.
           intros.
-          admit.
-        + admit.
+          eapply approximates_sub; eauto.
+        + eapply dmut_bind_sound. admit. admit.
+          apply dmut_assume_formula_sound.
+          intros.
+          eapply approximates_sub; eauto.
       - admit.
       - intros. apply dmut_bind_sound. admit. admit.
         apply IHasn1. intros.
-        (*  NOOOOOOOOOOOOO 😢😢  *)
-        intros ? ? ? ? ?. eapply IHasn2. admit.
-        admit.
+        eapply approximates_sub; eauto.
       - apply dmut_fresh_sound.
         + admit.
         + intros. apply IHasn.
@@ -626,37 +713,12 @@ Module Soundness
     Opaque dmut_wp.
     Opaque scmut_wp.
 
-    Section WithSemantics.
+    Section Leftovers.
 
       Context `{HL: IHeaplet L} {SLL: ISepLogicLaws L}.
 
       Definition interpret_heap {Σ} (ι : SymInstance Σ) (h : SymbolicHeap Σ) : L :=
         List.fold_right (fun c h => ASS.inst_chunk ι c ∧ h) ltrue h.
-
-      Ltac sauto :=
-        repeat
-          match goal with
-          | [ |- ?P ⊢ ?P ] =>
-            apply entails_refl
-          | [ |- ?P ∧ _ ⊢ ?P ∧ _ ] =>
-            apply land_right; [ apply land_left1, entails_refl | idtac ]
-          | [ |- _ ⊢ _ ∧ !!(?x = ?x) ] =>
-            apply land_right; [ idtac | apply lprop_right; reflexivity ]
-          | [ |- !! _ ⊢ _ ] =>
-            apply lprop_right; intro
-          | [ H: ?P |- _ ⊢ !!?P ] =>
-            apply lprop_right; exact H
-          end.
-
-      Local Ltac sound_inster :=
-        match goal with
-        | [ IH: outcome_satisfy (dmut_exec ?s _ _) |-
-            outcome_satisfy (dmut_exec ?s _ _) _ ] =>
-          refine (outcome_satisfy_monotonic _ _ IH); clear IH
-        | [ IH: context[_ -> outcome_satisfy (dmut_exec ?s _ _) _] |-
-            outcome_satisfy (dmut_exec ?s _ _) _ ] =>
-          microsail_insterU (fail) IH; refine (outcome_satisfy_monotonic _ _ IH); clear IH
-        end.
 
       Transparent subst SubstEnv.
       Lemma subst_lookup {Γ Σ Σ' x σ} (xInΓ : (x ∶ σ)%ctx ∈ Γ) (ζ : Sub Σ Σ') (δ : SymbolicLocalStore Γ Σ) :
@@ -692,72 +754,7 @@ Module Soundness
         all: induction es; cbn in *; destruct_conjs; f_equal; auto.
       Qed.
 
-      Local Opaque inst_heap.
-
-      Opaque env_tail.
-
-      Notation "'dmutres_pathcondition' res" := (symbolicstate_pathcondition (dmutres_result_state res)) (at level 10).
-      Notation "'dmutres_heap' res" := (symbolicstate_heap (dmutres_result_state res)) (at level 10).
-      Notation "'dmutres_localstore' res" := (symbolicstate_localstore (dmutres_result_state res)) (at level 10).
-
-      Lemma dmut_exec_sound {Γ σ} (POST : Lit σ -> LocalStore Γ -> L) (s : Stm Γ σ) :
-        forall Σ0 Σ1  (ι : SymInstance Σ1) (ζ1 : Sub Σ0 Σ1) (pc1 : PathCondition Σ1) (δ1 : SymbolicLocalStore Γ Σ1) (h1 : SymbolicHeap Σ1),
-          let δ       := inst ι δ1 in
-          let pre__pc   := inst_pathcondition ι pc1 in
-          let pre__heap := interpret_heap ι h1 in
-          outcome_satisfy
-            (dmut_exec s ζ1 (MkSymbolicState pc1 δ1 h1))
-            (fun '(@MkDynMutResult _ _ _ Σ2 ζ2 t (MkSymbolicState pc2 δ2 h2)) =>
-               forall (ι' : SymInstance Σ2),
-                 ι = env_map (fun _ => inst_term ι') ζ2 ->
-                 let post__pc   := inst_pathcondition ι' pc2 in
-                 let post__heap := interpret_heap ι' h2 in
-                 !! post__pc ∧ post__heap ⊢ POST (inst ι' t) (inst ι' δ2)) ->
-          pre__pc ->
-          outcome_satisfy
-            (scmut_exec s (MkSCState δ (inst ι h1)))
-            (fun '(MkSCMutResult v2 (MkSCState δ2 h2)) =>
-               SCMUT.inst_scheap h2 ⊢ POST v2 δ2).
-      Proof.
-        intros ? ? ? ? ? ? ?; cbn.
-        revert pc1 h1.
-        induction s.
-
-        - cbn. intros.
-          assert (ι = env_map (fun b : 𝑺 * Ty => inst_term ι) (sub_id Σ1)) as Heqι by admit.
-          specialize (H ι Heqι); clear Heqι.
-          refine (entails_trans _ _ _ _ H).
-          apply land_right.
-          + now apply lprop_right.
-          + admit.
-
-        - cbn. intros.
-          assert (ι = env_map (fun b : 𝑺 * Ty => inst_term ι) (sub_id Σ1)) as Heqι by admit.
-          specialize (H ι Heqι); clear Heqι.
-          change (env_map (fun (b : 𝑿 * Ty) (t : Term Σ1 (snd b)) => inst_term ι t) δ1) with
-              (inst ι δ1).
-          rewrite eval_exp_inst.
-          refine (entails_trans _ _ _ _ H).
-          apply land_right.
-          + now apply lprop_right.
-          + admit.
-
-        - repeat (unfold dmut_bind_right, dmut_sub, dmut_bind, scmut_bind,
-                  scmut_bind_left; cbn).
-          repeat
-            (repeat setoid_rewrite outcome_satisfy_bind;
-             repeat setoid_rewrite outcome_satisfy_map; cbn).
-          intros.
-
-      Admitted.
-
-      Lemma dmut_contract_sound {Δ τ} (c : SepContract Δ τ) (body : Stm Δ τ) :
-        ValidContractDynMut c body ->
-        ValidContract c body.
-      Proof.
-      Admitted.
-
-    End  WithSemantics.
+    End Leftovers.
 
   End DynMutV1Soundness.
 
